heap_lang/locales_helpers_hl.v
@@ -1,6 +1,7 @@
 From fairness Require Import locales_helpers utils_sets.
 From heap_lang Require Export lang tactics notation.
 
+Close Scope Z. 
   
 Lemma from_locale_from_lookup tp0 tp tid e :
   from_locale_from tp0 tp tid = Some e <-> (tp !! (tid - length tp0)%nat = Some e ∧ (length tp0 <= tid)%nat).
@@ -85,33 +86,192 @@ Proof.
   rewrite (length_upd_middle e1 e2). set_solver.
 Qed. 
 
+  (* TODO: move the lemmas below to appropriate places *)
+  (* TODO: this is pretty much the definition of locales_of_list *)
+  Lemma locales_of_list_from_locales t0 (es : list expr):
+    locales_of_list_from t0 es = map (fun '(l, e) => locale_of l e) (prefixes_from t0 es).
+  Proof using. set_solver. Qed. 
+
+  (* TODO: this is pretty much the definition of locales_of_list *)
+  Lemma locales_of_list_locales (es : list expr) :    
+    locales_of_list es = map (fun '(l, e) => locale_of l e) (prefixes es).
+  Proof using. set_solver. Qed. 
+
+  (* TODO: move *)
+  Lemma prefixes_from_ith_length (t0 t: list expr) pf i
+    (ITH: prefixes_from t0 t !! i = Some pf):
+    length pf.1 = length t0 + i.
+  Proof using.
+    clear -ITH. 
+    generalize dependent t0. generalize dependent i. generalize dependent pf.
+    induction t.
+    { intros. simpl. destruct t0; done. }
+    intros. destruct i.
+    { simpl in ITH. inversion ITH. subst. simpl. lia. }
+    simpl in ITH. apply IHt in ITH.
+    rewrite length_app /= in ITH. lia.
+  Qed.
+
+  Lemma prefixes_ith_length (t: list expr) pf i
+    (ITH: prefixes t !! i = Some pf):
+    length pf.1 = i. 
+  Proof using.
+    apply prefixes_from_ith_length in ITH. by rewrite ITH.
+  Qed.
+
+  Lemma from_locale_from_locale_of t0 t1 t2 e:
+    from_locale_from t0 (t1 ++ e :: t2) (locale_of (t0 ++ t1) e) = Some e.
+  Proof using.
+    apply from_locale_from_lookup.
+    rewrite /locale_of. rewrite length_app. simpl.
+    split; [| lia].
+    rewrite Nat.add_sub'. by apply list_lookup_middle.
+  Qed.
+
+  (* TODO: find existing *)
+  Lemma locales_equiv_from_of_list_from (tp1 tp2: list expr) tp01 tp02:
+    locales_equiv_from tp01 tp02 tp1 tp2 <-> locales_of_list_from tp01 tp1 = locales_of_list_from tp02 tp2.
+  Proof using.
+    rewrite !locales_of_list_from_locales.    
+    generalize dependent tp2. generalize dependent tp01. generalize dependent tp02. 
+    induction tp1.
+    { intros. simpl.
+      split; intros EQUIV.
+      - destruct tp2; inversion EQUIV. done.
+      - destruct tp2; [| done]. done. }
+    intros. simpl. split.
+    - intros EQUIV. inversion EQUIV; subst.
+      simpl. destruct y.
+      destruct tp2; [done| ].
+      simpl in H1. inversion H1. subst.
+      f_equal; [done| ].
+      by apply IHtp1.
+    - intros EQ. destruct tp2; [done| ].
+      simpl in EQ. inversion EQ.
+      simpl. econstructor; try done.
+      eapply IHtp1; eauto.
+  Qed.
+
+  (* TODO: find existing *)
+  Lemma locales_equiv_of_list (tp1 tp2: list expr):
+    locales_equiv tp1 tp2 <-> locales_of_list tp1 = locales_of_list tp2.
+  Proof using. apply locales_equiv_from_of_list_from. Qed.
+
+  Lemma locales_of_cfg_equiv tp1 tp2 σ1 σ2
+    (EQUIV: locales_equiv tp1 tp2):
+    locales_of_cfg (tp1, σ1) = locales_of_cfg (tp2, σ2).
+  Proof using.
+    rewrite /locales_of_cfg. simpl.
+    apply locales_equiv_of_list in EQUIV. by rewrite EQUIV.
+  Qed.
+
+  Lemma locales_of_cfg_ext tp1 ef σ:
+    locales_of_cfg (tp1 ++ [ef], σ) = locales_of_cfg (tp1, σ) ∪ {[ locale_of tp1 ef ]}.
+  Proof using.
+    rewrite /locales_of_cfg. simpl.
+    rewrite locales_of_list_locales.
+    rewrite prefixes_from_app map_app. simpl.
+    rewrite list_to_set_app_L. set_solver.
+  Qed. 
+
+  Lemma step_fork_locales_equiv c1 c2
+    (LOCALES_EQUIV: locales_equiv c1.1 c2.1):
+  step_fork c1 c2 = None.
+  Proof using.
+    rewrite /step_fork.
+    destruct c1, c2.
+    erewrite (locales_of_cfg_equiv l); eauto.
+    simpl. apply gset_pick_None.
+    apply difference_diag_L.
+  Qed.
+
+  Lemma step_fork_fork tp1 tp2 ef σ1 σ2
+    (EQUIV: locales_equiv tp1 tp2):
+    step_fork (tp1, σ1) (tp2 ++ [ef], σ2) = Some (locale_of tp1 ef).
+  Proof using.
+    rewrite /step_fork.
+    rewrite locales_of_cfg_ext. rewrite difference_union_distr_l_L.
+    erewrite (locales_of_cfg_equiv tp1); [| done].
+    erewrite difference_diag_L.
+    rewrite difference_disjoint_L.
+    2: { apply disjoint_singleton_l.
+         rewrite locales_of_cfg_simpl. rewrite /locale_of.
+         intros ?%elem_of_set_seq. simpl in H. lia. }
+    rewrite union_empty_l_L. simpl. rewrite gset_pick_singleton.
+    f_equal. rewrite /locale_of. apply Forall2_length in EQUIV.
+    rewrite !prefixes_from_length in EQUIV. done.
+  Qed.
+
+  Lemma step_fork_hl t1 t2 e e' efs σ σ'
+    (c := (t1 ++ e :: t2, σ))
+    (c' := (t1 ++ e' :: t2 ++ efs, σ'))
+    (STEP: locale_step c (Some (locale_of t1 e)) c'):
+    step_fork c c' = None /\ efs = [] \/ exists ef, efs = [ef] /\ step_fork c c' = Some (locale_of c.1 ef).
+  Proof using.
+    inversion STEP; subst. subst c c'.
+    rewrite /locale_of in H.
+    inversion H0. subst. 
+    assert (t0 = t1 /\ e1 = e /\ t3 = t2 /\ e2 = e' /\ efs0 = efs) as (-> & -> & -> & -> & ->). 
+    { by list_simplifier. }
+    simpl in H3. clear H H0 H4 H1.
+    inversion H3. subst. simpl in *.
+    inversion H1; subst.
+    all: try by (left; split; [| reflexivity];
+                 apply step_fork_locales_equiv; rewrite app_nil_r;
+                 apply locales_equiv_middle). 
+    right. eexists. split; eauto.
+    rewrite app_comm_cons. rewrite app_assoc. 
+    rewrite step_fork_fork; [done| ].
+    apply locales_equiv_middle. done.
+  Qed.
+
+Lemma locale_step_step_fork_exact c1 c2 τ
+  (STEP: locale_step c1 (Some τ) c2):
+  locales_of_cfg c2 = locales_of_cfg c1 ∪ from_option singleton ∅ (step_fork c1 c2).
+Proof using.
+  inversion STEP. subst.
+  eapply step_fork_hl in STEP.
+  destruct STEP as [[-> ->] | (? & -> & ->)].
+  - rewrite app_nil_r. simpl.
+    rewrite union_empty_r_L. apply locales_of_cfg_equiv.
+    by apply locales_equiv_middle.
+  - simpl. rewrite -locales_of_cfg_ext.
+    apply locales_of_cfg_equiv.
+    rewrite -app_assoc. rewrite -app_comm_cons.   
+    by apply locales_equiv_middle.
+Qed.
+
+Lemma step_fork_difference c1 c2 τ
+  (SF: step_fork c1 c2 = Some τ):
+  τ ∈ locales_of_cfg c2 ∖ locales_of_cfg c1.
+Proof using.
+  rewrite /step_fork in SF. apply gset_pick_Some in SF. set_solver.
+Qed.
+
 Lemma locale_step_fresh_exact c1 c2 τ τ'
   (STEP: locale_step c1 (Some τ) c2)
   (FRESH: τ' ∈ locales_of_cfg c2 ∖ locales_of_cfg c1):
   locales_of_cfg c2 = locales_of_cfg c1 ∪ {[ τ' ]} /\ τ' ∉ locales_of_cfg c1.
-Proof.
-  inversion STEP. subst.
-  revert FRESH.
-  
-  rewrite !locales_of_cfg_simpl. 
-  rewrite app_comm_cons. rewrite app_assoc. rewrite app_length.
-  rewrite -!list_to_set_seq. rewrite seq_app. simpl. 
-  rewrite list_to_set_app_L. rewrite !list_to_set_seq.
-  
-  rewrite (length_upd_middle e2 e1). remember (length (t1 ++ e1 :: t2)) as N.
-  rewrite -HeqN. remember (set_seq 0 N) as D. 
-  
-  rewrite difference_union_distr_l_L. rewrite subseteq_empty_difference; [| done].
-  rewrite union_empty_l. intros [DOM2 NDOM1]%elem_of_difference.
-  split; [| done].
-  f_equal.
-  
-  assert (¬ (efs = [])) as FORK.
-  { intros NOFORK. inversion H3. subst. inversion H1; subst; done. }
-  inversion H3. subst. inversion H1; subst; try done.
-  simpl in DOM2. rewrite union_empty_r in DOM2. apply elem_of_singleton in DOM2.
-  simpl. set_solver.
-Qed.            
+Proof using.
+  erewrite locale_step_step_fork_exact; eauto.
+  inversion STEP. subst. apply step_fork_hl in STEP.
+  destruct STEP as [[-> ->] | (? & -> & ->)].
+  - rewrite app_nil_r in FRESH.
+    erewrite locales_of_cfg_equiv in FRESH.
+    { erewrite difference_diag_L in FRESH. set_solver. }
+    by apply locales_equiv_middle.
+  - simpl. revert FRESH. 
+    rewrite app_comm_cons app_assoc. 
+    rewrite locales_of_cfg_ext. 
+    rewrite difference_union_distr_l_L. 
+    erewrite locales_of_cfg_equiv.
+    1: erewrite difference_diag_L.
+    2: { by apply locales_equiv_middle. }
+    rewrite union_empty_l_L. intros [->%elem_of_singleton ?]%elem_of_difference.
+    split; auto.
+    do 2 f_equal.
+    rewrite /locale_of. rewrite !length_app. simpl. lia.
+Qed.
 
 Lemma locale_step_fork_Some c1 τ c2 τ'
   (STEP: locale_step c1 (Some τ) c2)
